{
 "cells": [
  {
   "cell_type": "markdown",
   "metadata": {},
   "source": [
    "# 1. Sick or Healthy\n",
    "We will now look at a model that examines our state of healthiness vs. being sick. Keep in mind that this is very much like something you could do in real life. If you wanted to model a certain situation or environment, we could take some data that we have gathered, build a maximum likelihood model on it, and do things like study the properties that emerge from the model, or make predictions from the model, or generate the next most likely state. \n",
    "\n",
    "Let's say we have 2 states: **sick** and **healthy**. We know that we spend most of our time in a healthy state, so the probability of transitioning from healthy to sick is very low:\n",
    "\n",
    "#### $$p(sick \\; | \\; healthy) = 0.005$$\n",
    "\n",
    "Hence, the probability of going from healthy to healthy is:\n",
    "\n",
    "#### $$p(healthy \\; | \\; healthy) = 0.995$$\n",
    "\n",
    "Now, on the other hand the probability of going from sick to sick is also very high. This is because if you just got sick yesterday then you are very likely to be sick tomorrow.\n",
    "\n",
    "#### $$p(sick \\; | \\; sick) = 0.8$$\n",
    "\n",
    "However, the probability of transitioning from sick to healthy should be higher than the reverse, because you probaably won't stay sick for as long as you would stay healthy:\n",
    "\n",
    "#### $$p(healthy \\; | \\; sick) = 0.02$$\n",
    "\n",
    "We have now fully defined our state transition matrix, and we can now do some calculations. \n",
    "\n",
    "## 1.1 Example Calculations\n",
    "### 1.1.1 \n",
    "What is the probability of being healthy for 10 days in a row, given that we already start out as healthy? Well that is:\n",
    "\n",
    "#### $$p(healthy \\; 10 \\; days \\; in \\; a \\; row \\; | \\; healthy \\; at \\; t=0) = 0.995^9 = 95.6 \\%$$\n",
    "\n",
    "How about the probability of being healthy for 100 days in a row? \n",
    "\n",
    "#### $$p(healthy \\; 100 \\; days \\; in \\; a \\; row \\; | \\; healthy \\; at \\; t=0) = 0.995^99 = 60.9 \\%$$"
   ]
  },
  {
   "cell_type": "markdown",
   "metadata": {
    "collapsed": true
   },
   "source": [
    "---\n",
    "\n",
    "<br>\n",
    "# 2. Expected Number of Continuously Sick Days\n",
    "We can now look at the expected number of days that you would remain in the same state (e.g. how many days would you expect to stay sick given the model?). This is a bit more difficult than the last problem, but completely doable, only involving the mathematics of <a href=\"https://en.wikipedia.org/wiki/Geometric_series\">infinite sums</a>.\n",
    "\n",
    "First, we can look at the probability of being in state $i$, and going to state $i$ in the next state. That is just $A(i,i)$:\n",
    "\n",
    "#### $$p \\big(s(t)=i \\; | \\; s(t-1)=i \\big) = A(i, i)$$\n",
    "\n",
    "Now, what is the probability distribution that we actually want to calculate? How about we calculate the probability that we stay in state $i$ for $n$ transitions, at which point we move to another state:\n",
    "\n",
    "#### $$p \\big(s(t)!=i \\; | \\; s(t-1)=i \\big) = 1 - A(i, i)$$\n",
    "\n",
    "So, the joint probability that we are trying to model is:\n",
    "\n",
    "#### $$p\\big(s(1)=i, s(2)=i,...,s(n)=i, s(n+1) != i\\big) = A(i,i)^{n-1}\\big(1-A(i,i)\\big)$$\n",
    "\n",
    "In english this means that we are multiplying the transition probability of staying in the same state, $A(i,i)$, times the number of times we stayed in the same state, $n$, times $1 - A(i,i)$, the probability of transitioning from that state. This leaves us with an expected value for $n$ of:\n",
    "\n",
    "#### $$E(n) = \\sum np(n) = \\sum_{n=1..\\infty} nA(i,i)^{n-1}(1-A(i,i))$$\n",
    "\n",
    "Note, in the above equation $p(n)$ is the probability that we will see state $i$ $n-1$ times after starting from $i$ and then see a state that is not $i$. Also, we know that the expected value of $n$ should be the sum of all possible values of $n$ times $p(n)$. \n",
    "\n",
    "\n",
    "## 2.1 Expected $n$\n",
    "So, we can now expand this function and calculate the two sums separately. \n",
    "\n",
    "\n",
    "\n",
    "#### $$E(n) = \\sum_{n=1..\\infty}nA(i,i)^{n-1}(1 - A(i,i)) = \\sum nA(i, i)^{n-1} - \\sum nA(i,i)^n$$\n",
    "\n",
    "**First Sum**<br>\n",
    "With our first sum, we can say that:\n",
    "\n",
    "#### $$S = \\sum nA(i, i)^{n-1}$$\n",
    "\n",
    "#### $$S = 1 + 2A + 3A^2 + 4A^3+ ...$$\n",
    "\n",
    "And we can then multiply that sum, $S$, by $A$, to get:\n",
    "\n",
    "#### $$AS = a + 2A^2 + 3A^3 + 4A^4+...$$\n",
    "\n",
    "And then we can subtract $AS$ from $S$:\n",
    "\n",
    "#### $$S - AS = S'= 1 + A + A^2 + A^3+...$$\n",
    "\n",
    "This $S'$ is another infinite sum, but it is one that is much easier to solve! \n",
    "\n",
    "#### $$S'= 1 + A + A^2 + A^3+...$$\n",
    "\n",
    "And then $AS'$ is:\n",
    "\n",
    "#### $$AS' = A + A^2 + A^3+ + A^4 + ...$$\n",
    "\n",
    "Which, when we then do $S' - AS'$, we end up with:\n",
    "\n",
    "#### $$S' - AS' = 1$$\n",
    "#### $$S' = \\frac{1}{1 - A}$$\n",
    "\n",
    "And if we then substitute that value in for $S'$ above:\n",
    "\n",
    "#### $$S - AS = S'= 1 + A + A^2 + A^3+... = \\frac{1}{1 - A}$$\n",
    "#### $$S - AS = \\frac{1}{1 - A}$$\n",
    "#### $$S = \\frac{1}{(1 - A)^2}$$\n",
    "\n",
    "\n",
    "**Second Sum**<br>\n",
    "We can now look at our second sum:\n",
    "\n",
    "#### $$S = \\sum nA(i,i)^n$$\n",
    "\n",
    "#### $$S = 1A + 2A^2 + 3A^3 +...$$\n",
    "#### $$SA = 1A^2 + 2A^3 +...$$\n",
    "#### $$S - AS = S' = A + A^2 + A^3 + ...$$\n",
    "#### $$AS' = A^2 + A^3 + A^4 +...$$\n",
    "#### $$S' - AS' = A$$\n",
    "#### $$S' = \\frac{A}{1 - A}$$\n",
    "And we can plug back in $S'$ to get:\n",
    "\n",
    "#### $$S - AS = \\frac{A}{1 - A}$$\n",
    "#### $$S = \\frac{A}{(1 - A)^2}$$\n",
    "\n",
    "**Combine** <br>\n",
    "We can now combine these two sums as follows:\n",
    "\n",
    "#### $$E(n) = \\frac{1}{(1 - a)^2} - \\frac{a}{(1-a)^2}$$\n",
    "\n",
    "#### $$E(n) = \\frac{1}{1-a}$$\n",
    "\n",
    "**Calculate Number of Sick Days**<br>\n",
    "So, how do we calculate the correct number of sick days? That is just:\n",
    "\n",
    "#### $$\\frac{1}{1 - 0.8} = 5$$"
   ]
  },
  {
   "cell_type": "code",
   "execution_count": null,
   "metadata": {
    "collapsed": true
   },
   "outputs": [],
   "source": []
  },
  {
   "cell_type": "code",
   "execution_count": null,
   "metadata": {
    "collapsed": true
   },
   "outputs": [],
   "source": []
  },
  {
   "cell_type": "code",
   "execution_count": null,
   "metadata": {
    "collapsed": true
   },
   "outputs": [],
   "source": []
  }
 ],
 "metadata": {
  "kernelspec": {
   "display_name": "Python 3",
   "language": "python3",
   "name": "python3"
  },
  "language_info": {
   "codemirror_mode": {
    "name": "ipython",
    "version": 3
   },
   "file_extension": ".py",
   "mimetype": "text/x-python",
   "name": "python",
   "nbconvert_exporter": "python",
   "pygments_lexer": "ipython3",
   "version": "3.6.5"
  }
 },
 "nbformat": 4,
 "nbformat_minor": 2
}
